src/model/cut.v
@@ -1,0 +1,133 @@
+From Coq Require Import Lists.List.
+
+From VST Require Import floyd.sublist.
+From VST Require Import veric.base.
+
+From CertiGraph Require Import graph.graph_model.
+From CertiGraph Require Import lib.List_ext.
+
+From CertiGC Require Import model.constants.
+From CertiGC Require Import model.graph.
+From CertiGC Require Import model.heap.
+From CertiGC Require Import model.thread_info.
+From CertiGC Require Import model.util.
+
+
+Lemma cut_space__order: forall (sp : Space) (s : Z),
+    has_space sp s -> 0 <= space_allocated sp + s <= space_capacity sp.
+Proof. intros. pose proof (space__order sp). red in H. lia. Qed.
+
+Definition cut_space (sp: Space) (s: Z) (H: has_space sp s): Space := {|
+    space_base := space_base sp;
+    space_allocated := space_allocated sp + s;
+    space_capacity := space_capacity sp;
+    space_sh := space_sh sp;
+    space__order := cut_space__order sp s H;
+    space__upper_bound := space__upper_bound sp;
+|}.
+
+Lemma cut_heap_size:
+  forall (h : Heap) (i s : Z) (H : has_space (Znth i (heap_spaces h)) s),
+    0 <= i < Zlength (heap_spaces h) ->
+    Zlength (upd_Znth i (heap_spaces h) (cut_space (Znth i (heap_spaces h)) s H)) = MAX_SPACES.
+Proof. intros. rewrite upd_Znth_Zlength; [apply heap_spaces__size | assumption]. Qed.
+
+Definition cut_heap (h: Heap) (i s: Z) (H1: 0 <= i < Zlength (heap_spaces h))
+           (H2: has_space (Znth i (heap_spaces h)) s): Heap := {|
+  heap_spaces := upd_Znth i (heap_spaces h) (cut_space (Znth i (heap_spaces h)) s H2);
+  heap_spaces__size := cut_heap_size h i s H2 H1
+|}.
+
+Lemma heap_head_cut_thread_info: forall
+    h i s (H1: 0 <= i < Zlength (heap_spaces h)) (H2: has_space (Znth i (heap_spaces h)) s),
+    i <> 0 -> heap_head (cut_heap h i s H1 H2) = heap_head h.
+Proof.
+  intros. destruct (heap_head__cons h) as [hs1 [l1 [? ?]]].
+  destruct (heap_head__cons (cut_heap h i s H1 H2)) as [hs2 [l2 [? ?]]].
+  rewrite H3, H5. simpl in H4.
+  pose proof (split3_full_length_list
+                0 i _ _ H1 (Zminus_0_l_reverse (Zlength (heap_spaces h)))).
+  replace (i - 0) with i in H6 by lia. simpl in H6.
+  remember (firstn (Z.to_nat i) (heap_spaces h)) as ls1.
+  remember (skipn (Z.to_nat (i + 1)) (heap_spaces h)) as ls2.
+  assert (Zlength ls1 = i). {
+    rewrite Zlength_length by lia. subst ls1. apply firstn_length_le.
+    clear H5. rewrite Zlength_correct in H1. lia. }
+  rewrite H6 in H4 at 1. rewrite (upd_Znth_char _ _ _ _ _ H7) in H4.
+  rewrite H6 in H0. clear -H0 H4 H H7. destruct ls1.
+  - rewrite Zlength_nil in H7. exfalso. apply H. subst i. reflexivity.
+  - simpl in H0, H4. inversion H0. subst hs1. inversion H4. reflexivity.
+Qed.
+
+Definition cut_thread_info (t: thread_info) (i s: Z)
+           (H1: 0 <= i < Zlength (heap_spaces (ti_heap t)))
+           (H2: has_space (Znth i (heap_spaces (ti_heap t))) s) : thread_info :=
+  Build_thread_info (ti_heap_p t) (cut_heap (ti_heap t) i s H1 H2) (ti_args t)
+                    (arg_size t).
+
+Lemma cti_eq: forall t i s1 s2 (H1: 0 <= i < Zlength (heap_spaces (ti_heap t)))
+                     (Hs1: has_space (Znth i (heap_spaces (ti_heap t))) s1)
+                     (Hs2: has_space (Znth i (heap_spaces (ti_heap t))) s2),
+    s1 = s2 -> cut_thread_info t i s1 H1 Hs1 = cut_thread_info t i s2 H1 Hs2.
+Proof.
+  intros. unfold cut_thread_info. f_equal. subst s1. f_equal. apply proof_irr.
+Qed.
+
+
+Lemma cti_rest_gen_size:
+  forall t_info to s
+         (Hi : 0 <= Z.of_nat to < Zlength (heap_spaces (ti_heap t_info)))
+         (Hh : has_space (Znth (Z.of_nat to) (heap_spaces (ti_heap t_info))) s),
+  rest_gen_size t_info to =
+  rest_gen_size (cut_thread_info t_info (Z.of_nat to) s Hi Hh) to + s.
+Proof.
+  intros. unfold rest_gen_size. rewrite !nth_space_Znth. unfold cut_thread_info. simpl.
+  rewrite upd_Znth_same by assumption. simpl. lia.
+Qed.
+
+Lemma cti_space_not_eq: forall t_info i s n
+    (Hi : 0 <= i < Zlength (heap_spaces (ti_heap t_info)))
+    (Hh : has_space (Znth i (heap_spaces (ti_heap t_info))) s),
+    (Z.of_nat n) <> i ->
+    nth_space (cut_thread_info t_info i s Hi Hh) n = nth_space t_info n.
+Proof.
+  intros. rewrite !nth_space_Znth. simpl.
+  pose proof (Nat2Z.is_nonneg n). remember (Z.of_nat n). clear Heqz.
+  remember (heap_spaces (ti_heap t_info)). destruct (Z_lt_le_dec z (Zlength l)).
+  - assert (0 <= z < Zlength l) by lia.
+    rewrite upd_Znth_diff; [reflexivity |assumption..].
+  - rewrite !Znth_overflow;
+      [reflexivity | | rewrite upd_Znth_Zlength by assumption]; lia.
+Qed.
+
+Lemma cti_space_eq: forall t_info i s
+    (Hi : 0 <= Z.of_nat i < Zlength (heap_spaces (ti_heap t_info)))
+    (Hh : has_space (Znth (Z.of_nat i) (heap_spaces (ti_heap t_info))) s),
+    nth_space (cut_thread_info t_info (Z.of_nat i) s Hi Hh) i =
+    cut_space (Znth (Z.of_nat i) (heap_spaces (ti_heap t_info))) s Hh.
+Proof.
+  intros. rewrite nth_space_Znth. simpl. rewrite upd_Znth_same by assumption.
+  reflexivity.
+Qed.
+
+Lemma cti_gen_size: forall t_info i s n
+    (Hi : 0 <= i < Zlength (heap_spaces (ti_heap t_info)))
+    (Hh : has_space (Znth i (heap_spaces (ti_heap t_info))) s),
+    gen_size (cut_thread_info t_info i s Hi Hh) n =
+    gen_size t_info n.
+Proof.
+  intros. unfold gen_size. destruct (Z.eq_dec (Z.of_nat n) i).
+  - subst i. rewrite cti_space_eq. simpl. rewrite nth_space_Znth. reflexivity.
+  - rewrite cti_space_not_eq; [reflexivity | assumption].
+Qed.
+
+Lemma cti_space_base: forall t_info i s  n
+    (Hi : 0 <= i < Zlength (heap_spaces (ti_heap t_info)))
+    (Hh : has_space (Znth i (heap_spaces (ti_heap t_info))) s),
+    space_base (nth_space (cut_thread_info t_info i s Hi Hh) n) =
+    space_base (nth_space t_info n).
+Proof.
+  intros. destruct (Z.eq_dec (Z.of_nat n) i).
+  - subst i. rewrite cti_space_eq. simpl. rewrite nth_space_Znth. reflexivity.
+  - rewrite cti_space_not_eq; [reflexivity | assumption].
+Qed.
